theories/util/update.v
@@ -18,17 +18,33 @@ Proof. by elim n; [apply _|]=>/= *??->. Qed.
 Lemma step_fupdN_full_intro E n P : P ={E}▷=∗^n P.
 Proof. iIntros "?". by iApply step_fupdN_intro. Qed.
 
-Lemma step_fupdN_nmono E m n P : m ≤ n → (|={E}▷=>^m P) -∗ (|={E}▷=>^n P).
+Lemma step_fupdN_nmono m n P E : m ≤ n → (|={E}▷=>^m P) -∗ (|={E}▷=>^n P).
 Proof.
   move: n. elim m=>/= [|?]; [iIntros; by iApply step_fupdN_full_intro|].
   move=> IH ? /succ_le [?[->Le]]/=. iIntros "?". by iApply IH.
 Qed.
 
-Lemma step_fupdN_combine n E P Q :
+Lemma step_fupdN_combine n P Q E :
   (|={E}▷=>^n P) -∗ (|={E}▷=>^n Q) -∗ (|={E}▷=>^n (P ∗ Q)).
 Proof.
   elim n=>/= [|?]; [iIntros; by iFrame|]. iIntros (IH) ">UpdP >UpdQ !>!>".
   by iMod (IH with "UpdP UpdQ").
+Qed.
+
+Lemma step_fupdN_combine_max m n P Q E :
+  (|={E}▷=>^m P) -∗ (|={E}▷=>^n Q) -∗ (|={E}▷=>^(m `max` n) (P ∗ Q)).
+Proof.
+  set l := m `max` n. rewrite (step_fupdN_nmono _ l P); [|lia].
+  rewrite (step_fupdN_nmono _ l Q); [|lia]. apply step_fupdN_combine.
+Qed.
+
+Lemma step_fupdN_with_emp n P E :
+  (|={E}=> |={E}▷=>^n |={E}=> P) -∗ (|={E, ∅}=> |={∅}▷=>^n |={∅, E}=> P).
+Proof.
+  elim: n=> /=[|n IH].
+  - iIntros ">>Upd". iApply fupd_mask_intro_subseteq; [set_solver|done].
+  - iIntros ">>Upd". iApply fupd_mask_intro; [set_solver|].
+    iIntros "Close !>!>". iDestruct (IH with "Upd") as "?". by iMod "Close".
 Qed.
 
 End lemmas.
